Implement CT64 version of GHASH

code/aes-gcm/Hacl.AES_128_GCM.CT64.fst
@@ -1,20 +1,21 @@
-module Hacl.AES_128_GCM.NI
-
+module Hacl.AES_128_GCM.CT64
 open FStar.HyperStack
 open FStar.HyperStack.All
-
 open Lib.IntTypes
 open Lib.Buffer
 open Lib.ByteBuffer
-open Lib.IntVector
 
-open Hacl.AES_128.CTR32.NI
-open Hacl.Gf128.NI
+open Hacl.AES_128.CTR32.BitSlice
+open Hacl.Gf128.CT64
 
 module ST = FStar.HyperStack.ST
 
-#set-options "--z3rlimit 50"
-type aes_gcm_ctx = lbuffer (vec_t U128 1) 18ul
+
+#reset-options "--z3rlimit 1500 --max_fuel 1"
+
+let aes_gcm_ctx_len = 116ul
+
+type aes_gcm_ctx = lbuffer uint64 aes_gcm_ctx_len
 
 inline_for_extraction noextract
 val aes128_gcm_compute_iv:
@@ -29,10 +30,11 @@ let aes128_gcm_compute_iv ctx iv_len iv =
   push_frame();
   if (iv_len =. size 12) then (
     let tag_mix = create 16ul (u8 0) in
-    let aes_ctx = sub ctx (size 0) (size 12) in
+    let aes_ctx = sub ctx (size 0) (size 96) in
     aes128_set_nonce aes_ctx iv;
     aes128_key_block tag_mix aes_ctx (u32 1);
-    ctx.(17ul) <- vec_load_le U128 1 tag_mix;
+    ctx.(114ul) <- uint_from_bytes_le #U64 (sub tag_mix 0ul 8ul);
+    ctx.(115ul) <- uint_from_bytes_le #U64 (sub tag_mix 8ul 8ul);
     pop_frame();
     u32 2)
   else (
@@ -40,9 +42,10 @@ let aes128_gcm_compute_iv ctx iv_len iv =
     let tag_iv = create 16ul (u8 0) in
     let size_iv = create 16ul (u8 0) in
     let tag_mix = create 16ul (u8 0) in
-    let aes_ctx = sub ctx (size 0) (size 12) in
-    let gcm_ctx = sub ctx (size 12) (size 5) in
-    vec_store_be gcm_key gcm_ctx.(size 4);
+    let aes_ctx = sub ctx (size 0) (size 96) in
+    let gcm_ctx = sub ctx (size 96) (size 18) in
+    uint_to_bytes_be #U64 (sub gcm_key (size 8) (size 8)) gcm_ctx.(size 8);
+    uint_to_bytes_be #U64 (sub gcm_key (size 0) (size 8)) gcm_ctx.(size 9);
     ghash tag_iv iv_len iv gcm_key;
     uint_to_bytes_be #U64 (sub size_iv (size 8) (size 8)) (to_u64 (iv_len *. 8ul));
     let h0 = ST.get() in
@@ -52,7 +55,8 @@ let aes128_gcm_compute_iv ctx iv_len iv =
     aes128_set_nonce aes_ctx (sub tag_iv (size 0) (size 12));
     let ctr = uint_from_bytes_be #U32 (sub tag_iv (size 12) (size 4)) in
     aes128_key_block tag_mix aes_ctx ctr;
-    ctx.(17ul) <- vec_load_le U128 1 tag_mix;
+    ctx.(114ul) <- uint_from_bytes_le #U64 (sub tag_mix 0ul 8ul);
+    ctx.(115ul) <- uint_from_bytes_le #U64 (sub tag_mix 8ul 8ul);
     let ctr = ctr +. u32 1 in
     pop_frame();
     ctr)
@@ -68,14 +72,14 @@ let aes128_gcm_init ctx key =
   push_frame();
   let gcm_key = create 16ul (u8 0) in
   let nonce0 = create 12ul (u8 0) in
-  let aes_ctx = sub ctx (size 0) (size 12) in
-  let gcm_ctx = sub ctx (size 12) (size 5) in
+  let aes_ctx = sub ctx (size 0) (size 96) in
+  let gcm_ctx = sub ctx (size 96) (size 18) in
+  admit();
   aes128_init aes_ctx key nonce0;
   aes128_key_block gcm_key aes_ctx (u32 0);
   gcm_init gcm_ctx gcm_key;
   pop_frame()
 
-#reset-options "--z3rlimit 500 --max_fuel 1"
 
 val aes128_gcm_encrypt:
     ctx: aes_gcm_ctx
@@ -89,10 +93,10 @@ val aes128_gcm_encrypt:
   Stack unit
   (requires (fun h -> live h out /\ live h text /\ live h aad /\ live h iv /\ live h ctx
                  /\ disjoint out ctx
-                 /\ disjoint out text
-                 /\ disjoint out aad
                  /\ disjoint ctx text
                  /\ disjoint ctx aad
+                 /\ disjoint out text
+                 /\ disjoint out aad
                  /\ disjoint iv out
                  /\ disjoint iv text
                  /\ disjoint iv aad
@@ -100,27 +104,33 @@ val aes128_gcm_encrypt:
   (ensures (fun h0 _ h1 -> modifies2 out ctx h0 h1))
 
 let aes128_gcm_encrypt ctx len out text aad_len aad iv_len iv =
-  admit();
   push_frame();
-  let ctr = aes128_gcm_compute_iv ctx iv_len iv in
-  let cip = sub out (size 0) len in
-  let aes_ctx = sub ctx (size 0) (size 12) in
-  aes128_ctr len cip text aes_ctx ctr;
-  let gcm_ctx = sub ctx (size 12) (size 5) in
-  let tag_mix = ctx.(17ul) in
-  gcm_ctx.(0ul) <- vec_zero U128 1;
-  gcm_update_padded gcm_ctx aad_len aad;
-  gcm_update_padded gcm_ctx len cip;
   let tmp = create 16ul (u8 0) in
+  let cip = sub out (size 0) len in
+  let aes_ctx = sub ctx (size 0) (size 96) in
+  let gcm_ctx = sub ctx (size 96) (size 18) in
+  let tag_mix = sub ctx (size 114) (size 2) in
+  admit();
+  let ctr = aes128_gcm_compute_iv ctx iv_len iv in
+  aes128_ctr len cip text aes_ctx ctr;
+  gcm_ctx.(0ul) <- u64 0;
+  gcm_ctx.(1ul) <- u64 0;
+  gcm_update_blocks_padded gcm_ctx aad_len aad;
+  gcm_update_blocks_padded gcm_ctx len cip;
   uint_to_bytes_be #U64 (sub tmp (size 0) (size 8)) (to_u64 (aad_len *. 8ul));
   uint_to_bytes_be #U64 (sub tmp (size 8) (size 8)) (to_u64 (len *. 8ul));
   gcm_update_blocks gcm_ctx (size 16) tmp;
   gcm_emit tmp gcm_ctx;
-  let tmp_vec = vec_load_le U128 1 tmp in
-  let tmp_vec = vec_xor tmp_vec tag_mix in
-  vec_store_le (sub out len (size 16)) tmp_vec;
+  let tmp0 = uint_from_bytes_le #U64 (sub tmp 0ul 8ul) in
+  let tmp1 = uint_from_bytes_le #U64 (sub tmp 8ul 8ul) in
+  let tmp0 = tmp0 ^. tag_mix.(0ul) in
+  let tmp1 = tmp1 ^. tag_mix.(1ul) in
+  uint_to_bytes_le #U64 (sub out len 8ul) tmp0;
+  uint_to_bytes_le #U64 (sub out (len +. 8ul) 8ul) tmp1;
   pop_frame()
 
+
+#reset-options "--z3rlimit 1500 --max_fuel 1"
 
 val aes128_gcm_decrypt:
     ctx: aes_gcm_ctx
@@ -134,10 +144,10 @@ val aes128_gcm_decrypt:
   Stack bool
   (requires (fun h -> live h out /\ live h cipher /\ live h aad /\ live h iv /\ live h ctx
                  /\ disjoint out ctx
-                 /\ disjoint out cipher
-                 /\ disjoint out aad
                  /\ disjoint ctx cipher
                  /\ disjoint ctx aad
+                 /\ disjoint out cipher
+                 /\ disjoint out aad
                  /\ disjoint iv out
                  /\ disjoint iv cipher
                  /\ disjoint iv aad
@@ -154,20 +164,24 @@ let aes128_gcm_decrypt ctx len out cipher aad_len aad iv_len iv =
   let ciphertext = sub cipher 0ul len in
   let tag = sub cipher len (size 16) in
   let ctr = aes128_gcm_compute_iv ctx iv_len iv in
-  let aes_ctx = sub ctx (size 0) (size 12) in
-  let gcm_ctx = sub ctx (size 12) (size 5) in
-  let tag_mix = ctx.(17ul) in
+  let aes_ctx = sub ctx (size 0) (size 96) in
+  let gcm_ctx = sub ctx (size 96) (size 18) in
+  let tag_mix = sub ctx (size 114) (size 2) in
   let h1 = ST.get () in
-  gcm_ctx.(0ul) <- vec_zero U128 1;
-  gcm_update_padded gcm_ctx aad_len aad;
-  gcm_update_padded gcm_ctx len ciphertext;
+  gcm_ctx.(0ul) <- u64 0;
+  gcm_ctx.(1ul) <- u64 0;
+  gcm_update_blocks_padded gcm_ctx aad_len aad;
+  gcm_update_blocks_padded gcm_ctx len ciphertext;
   uint_to_bytes_be #U64 (sub text (size 0) (size 8)) (to_u64 (aad_len *. size 8));
   uint_to_bytes_be #U64 (sub text (size 8) (size 8)) (to_u64 (len *. size 8));
   gcm_update_blocks gcm_ctx (size 16) text;
   gcm_emit text gcm_ctx;
-  let text_vec = vec_load_le U128 1 text in
-  let text_vec = vec_xor text_vec tag_mix in
-  vec_store_le text text_vec;
+  let text0 = uint_from_bytes_le #U64 (sub text 0ul 8ul) in
+  let text1 = uint_from_bytes_le #U64 (sub text 8ul 8ul) in
+  let text0 = text0 ^. tag_mix.(0ul) in
+  let text1 = text1 ^. tag_mix.(1ul) in
+  uint_to_bytes_le #U64 (sub text 0ul 8ul) text0;
+  uint_to_bytes_le #U64 (sub text 8ul 8ul) text1;
   let h7 = ST.get () in
   loop_nospec #h7 (size 16) result
     (fun i -> result.(0ul) <- result.(0ul) |. (text.(i) ^. tag.(i)));
