code/aes-gcm/Hacl.AES_256_GCM.NI.fst
@@ -8,7 +8,7 @@ open Lib.Buffer
 open Lib.ByteBuffer
 open Lib.IntVector
 
-open Hacl.AES_256.NI
+open Hacl.AES_256.CTR32.NI
 open Hacl.Gf128.NI
 
 module ST = FStar.HyperStack.ST
@@ -17,28 +17,63 @@ module ST = FStar.HyperStack.ST
 #set-options "--z3rlimit 50"
 type aes_gcm_ctx = lbuffer (vec_t U128 1) 22ul
 
+inline_for_extraction noextract
+val aes256_gcm_compute_iv:
+    ctx: aes_gcm_ctx
+  -> iv_len: size_t
+  -> iv: lbuffer uint8 iv_len ->
+  Stack uint32
+  (requires (fun h -> live h ctx /\ live h iv))
+  (ensures (fun h0 _ h1 -> modifies1 ctx h0 h1))
+
+let aes256_gcm_compute_iv ctx iv_len iv =
+  push_frame();
+  if (iv_len =. size 12) then (
+    let tag_mix = create 16ul (u8 0) in
+    let aes_ctx = sub ctx (size 0) (size 16) in
+    aes256_set_nonce aes_ctx iv;
+    aes256_key_block tag_mix aes_ctx (u32 1);
+    ctx.(21ul) <- vec_load_le U128 1 tag_mix;
+    pop_frame();
+    u32 2)
+  else (
+    let gcm_key = create 16ul (u8 0) in
+    let tag_iv = create 16ul (u8 0) in
+    let size_iv = create 16ul (u8 0) in
+    let tag_mix = create 16ul (u8 0) in
+    let aes_ctx = sub ctx (size 0) (size 16) in
+    let gcm_ctx = sub ctx (size 16) (size 5) in
+    vec_store_be gcm_key gcm_ctx.(size 4);
+    ghash tag_iv iv_len iv gcm_key;
+    uint_to_bytes_be #U64 (sub size_iv (size 8) (size 8)) (to_u64 (iv_len *. 8ul));
+    let h0 = ST.get() in
+    loop_nospec #h0 (size 16) size_iv
+      (fun i -> size_iv.(i) <- tag_iv.(i) ^. size_iv.(i));
+    ghash tag_iv (size 16) size_iv gcm_key;
+    aes256_set_nonce aes_ctx (sub tag_iv (size 0) (size 12));
+    let ctr = uint_from_bytes_be #U32 (sub tag_iv (size 12) (size 4)) in
+    aes256_key_block tag_mix aes_ctx ctr;
+    ctx.(21ul) <- vec_load_le U128 1 tag_mix;
+    let ctr = ctr +. u32 1 in
+    pop_frame();
+    ctr)
 
 val aes256_gcm_init:
     ctx: aes_gcm_ctx
-  -> key: lbuffer uint8 32ul
-  -> nonce: lbuffer uint8 12ul ->
+  -> key: lbuffer uint8 32ul ->
   Stack unit
-  (requires (fun h -> live h ctx /\ live h key /\ live h nonce))
+  (requires (fun h -> live h ctx /\ live h key))
   (ensures (fun h0 _ h1 -> modifies1 ctx h0 h1))
 
-let aes256_gcm_init ctx key nonce =
+let aes256_gcm_init ctx key =
   push_frame();
   let gcm_key = create 16ul (u8 0) in
-  let tag_mix = create 16ul (u8 0) in
   let nonce0 = create 12ul (u8 0) in
   let aes_ctx = sub ctx (size 0) (size 16) in
   let gcm_ctx = sub ctx (size 16) (size 5) in
   aes256_init aes_ctx key nonce0;
-  aes256_key_block gcm_key aes_ctx (size 0);
-  aes256_set_nonce aes_ctx nonce;
-  aes256_key_block tag_mix aes_ctx (size 1);
+  aes256_key_block gcm_key aes_ctx (u32 0);
   gcm_init gcm_ctx gcm_key;
-  ctx.(21ul) <- vec_load_le U128 1 tag_mix;
   pop_frame()
 
 #reset-options "--z3rlimit 500 --max_fuel 1"
@@ -49,24 +84,32 @@ val aes256_gcm_encrypt:
   -> out: lbuffer uint8 (len +. 16ul)
   -> text: lbuffer uint8 len
   -> aad_len: size_t
-  -> aad: lbuffer uint8 aad_len ->
+  -> aad: lbuffer uint8 aad_len
+  -> iv_len: size_t
+  -> iv: lbuffer uint8 iv_len ->
   Stack unit
-  (requires (fun h -> live h out /\ live h text /\ live h aad /\ live h ctx
+  (requires (fun h -> live h out /\ live h text /\ live h aad /\ live h iv /\ live h ctx
                  /\ disjoint out ctx
                  /\ disjoint out text
                  /\ disjoint out aad
                  /\ disjoint ctx text
-                 /\ disjoint ctx aad))
+                 /\ disjoint ctx aad
+                 /\ disjoint iv out
+                 /\ disjoint iv text
+                 /\ disjoint iv aad
+                 /\ disjoint iv ctx))
   (ensures (fun h0 _ h1 -> modifies2 out ctx h0 h1))
 
-let aes256_gcm_encrypt ctx len out text aad_len aad =
+let aes256_gcm_encrypt ctx len out text aad_len aad iv_len iv =
   admit();
   push_frame();
+  let ctr = aes256_gcm_compute_iv ctx iv_len iv in
   let cip = sub out (size 0) len in
   let aes_ctx = sub ctx (size 0) (size 16) in
-  aes256_ctr len cip text aes_ctx (size 2);
+  aes256_ctr len cip text aes_ctx ctr;
   let gcm_ctx = sub ctx (size 16) (size 5) in
   let tag_mix = ctx.(21ul) in
+  gcm_ctx.(0ul) <- vec_zero U128 1;
   gcm_update_padded gcm_ctx aad_len aad;
   gcm_update_padded gcm_ctx len cip;
   let tmp = create 16ul (u8 0) in
@@ -86,17 +129,23 @@ val aes256_gcm_decrypt:
   -> out: lbuffer uint8 len
   -> cipher: lbuffer uint8 (len +. 16ul)
   -> aad_len: size_t
-  -> aad: lbuffer uint8 aad_len ->
+  -> aad: lbuffer uint8 aad_len
+  -> iv_len: size_t
+  -> iv: lbuffer uint8 iv_len ->
   Stack bool
-  (requires (fun h -> live h out /\ live h cipher /\ live h aad /\ live h ctx
+  (requires (fun h -> live h out /\ live h cipher /\ live h aad /\ live h iv /\ live h ctx
                  /\ disjoint out ctx
                  /\ disjoint out cipher
                  /\ disjoint out aad
                  /\ disjoint ctx cipher
-                 /\ disjoint ctx aad))
+                 /\ disjoint ctx aad
+                 /\ disjoint iv out
+                 /\ disjoint iv cipher
+                 /\ disjoint iv aad
+                 /\ disjoint iv ctx))
   (ensures (fun h0 r h1 -> modifies2 out ctx h0 h1))
 
-let aes256_gcm_decrypt ctx len out cipher aad_len aad =
+let aes256_gcm_decrypt ctx len out cipher aad_len aad iv_len iv =
   admit();
   push_frame();
   let scratch = create 18ul (u8 0) in
@@ -105,10 +154,12 @@ let aes256_gcm_decrypt ctx len out cipher aad_len aad =
   let result = sub scratch 17ul 1ul in
   let ciphertext = sub cipher 0ul len in
   let tag = sub cipher len (size 16) in
+  let ctr = aes256_gcm_compute_iv ctx iv_len iv in
   let aes_ctx = sub ctx (size 0) (size 16) in
   let gcm_ctx = sub ctx (size 16) (size 5) in
   let tag_mix = ctx.(21ul) in
   let h1 = ST.get () in
+  gcm_ctx.(0ul) <- vec_zero U128 1;
   gcm_update_padded gcm_ctx aad_len aad;
   gcm_update_padded gcm_ctx len ciphertext;
   uint_to_bytes_be #U64 (sub text (size 0) (size 8)) (to_u64 (aad_len *. size 8));
@@ -126,7 +177,7 @@ let aes256_gcm_decrypt ctx len out cipher aad_len aad =
   let res8 = result.(0ul) in
   let r =
     if Lib.RawIntTypes.u8_to_UInt8 res8 = 0uy then (
-      aes256_ctr len out ciphertext aes_ctx (size 2);
+      aes256_ctr len out ciphertext aes_ctx ctr;
       true)
     else (
       let h9 = ST.get () in
