code/gf128/Hacl.Impl.Gf128.Generic.fst
@@ -255,7 +255,6 @@ let gf128_update_multi_add_mul_f #s pre nb len text b4 i acc =
   normalize4 acc b4 pre
 
 
-//NI
 #push-options "--max_fuel 1"
 inline_for_extraction noextract
 val gf128_update_multi_add_mul:
@@ -308,144 +307,6 @@ let gf128_update_multi_add_mul #s acc pre len text =
 #pop-options
 
 inline_for_extraction noextract
-val gf128_update_multi_mul_add_f:
-    #s:field_spec
-  -> pre:precomp s
-  -> nb:size_t
-  -> len:size_t{v nb == v len / 64 /\ 0 < v len /\ v len % 64 = 0}
-  -> text:lbuffer uint8 len
-  -> b4:felem4 s
-  -> i:size_t{v i < v nb}
-  -> acc:felem4 s ->
-  Stack unit
-  (requires fun h ->
-    live h pre /\ live h acc /\ live h text /\ live h b4 /\
-    disjoint acc pre /\ disjoint acc text /\ disjoint b4 acc /\
-    disjoint b4 text /\ disjoint b4 pre /\
-    precomp_inv_t h pre)
-  (ensures  fun h0 _ h1 ->
-    modifies2 acc b4 h0 h1 /\ precomp_inv_t h1 pre /\
-    feval4 h1 acc == LSeq.repeat_blocks_f #uint8 #Vec.elem4 64 (as_seq h0 text)
-      (Vec.gf128_update4_mul_add (get_r4321 h0 pre)) (v nb) (v i) (feval4 h0 acc))
-
-let gf128_update_multi_mul_add_f #s pre nb len text b4 i acc4 =
-  let tb = sub text (i *! 64ul) 64ul in
-  encode4 b4 tb;
-  fmul_r4 acc4 pre;
-  fadd4 acc4 b4
-
-
-inline_for_extraction noextract
-val load_acc:
-    #s:field_spec
-  -> acc:felem s
-  -> text:lbuffer uint8 64ul
-  -> acc4:felem4 s
-  -> b4:felem4 s ->
-  Stack unit
-  (requires fun h ->
-    live h acc /\ live h text /\ live h acc4 /\ live h b4 /\
-    disjoint acc4 text /\ disjoint acc4 acc /\ disjoint acc4 b4 /\
-    disjoint b4 text /\ disjoint b4 acc /\
-    feval4 h acc4 == LSeq.create 4 zero)
-  (ensures  fun h0 _ h1 -> modifies2 acc4 b4 h0 h1 /\
-    feval4 h1 acc4 == Vec.load_acc (as_seq h0 text) (feval h0 acc))
-
-let load_acc #s acc tb acc4 b4 =
-  let h0 = ST.get () in
-  update_sub acc4 0ul (felem_len s) acc;
-  let h1 = ST.get () in
-  assert (feval4 h1 acc4 == LSeq.create4 (feval h0 acc) zero zero zero);
-  encode4 b4 tb;
-  fadd4 acc4 b4
-
-
-#push-options "--max_fuel 1"
-inline_for_extraction noextract
-val gf128_update_multi_mul_add_loop:
-    #s:field_spec
-  -> pre:precomp s
-  -> len:size_t{v len % 64 = 0}
-  -> text:lbuffer uint8 len
-  -> acc4:felem4 s
-  -> b4:felem4 s ->
-  Stack unit
-  (requires fun h ->
-    live h acc4 /\ live h pre /\ live h text /\ live h b4 /\
-    disjoint acc4 pre /\ disjoint acc4 text /\ disjoint acc4 b4 /\
-    disjoint b4 text /\ disjoint b4 pre /\
-    precomp_inv_t h pre)
-  (ensures  fun h0 _ h1 ->
-    modifies2 acc4 b4 h0 h1 /\ precomp_inv_t h1 pre /\
-    feval4 h1 acc4 == LSeq.repeat_blocks_multi #uint8 #Vec.elem4 64
-      (as_seq h0 text) (Vec.gf128_update4_mul_add (get_r4321 h0 pre)) (feval4 h0 acc4))
-
-let gf128_update_multi_mul_add_loop #s pre len text acc4 b4 =
-  let nb = len /. 64ul in
-  let h0 = ST.get () in
-
-  LSeq.lemma_repeat_blocks_multi #uint8 #Vec.elem4 64 (as_seq h0 text)
-    (Vec.gf128_update4_mul_add (get_r4321 h0 pre)) (feval4 h0 acc4);
-
-  [@ inline_let]
-  let spec_fh h0 =
-    LSeq.repeat_blocks_f 64 (as_seq h0 text)
-      (Vec.gf128_update4_mul_add (get_r4321 h0 pre)) (v nb) in
-
-  [@ inline_let]
-  let inv h (i:nat{i <= v nb}) =
-    modifies2 acc4 b4 h0 h /\
-    live h pre /\ live h acc4 /\ live h text /\ live h b4 /\
-    disjoint acc4 pre /\ disjoint acc4 text /\ disjoint b4 acc4 /\
-    disjoint b4 text /\ disjoint b4 pre /\
-    precomp_inv_t h pre /\
-    feval4 h acc4 == Lib.LoopCombinators.repeati i (spec_fh h0) (feval4 h0 acc4) in
-
-  Lib.Loops.for (size 0) nb inv
-    (fun i ->
-      Lib.LoopCombinators.unfold_repeati (v nb) (spec_fh h0) (feval4 h0 acc4) (v i);
-      gf128_update_multi_mul_add_f #s pre nb len text b4 i acc4);
-
-  let h1 = ST.get () in
-  assert (feval4 h1 acc4 == Lib.LoopCombinators.repeati (v nb) (spec_fh h0) (feval4 h0 acc4))
-#pop-options
-
-
-#set-options "--z3rlimit 100"
-
-//PreComp
-inline_for_extraction noextract
-val gf128_update_multi_mul_add:
-    #s:field_spec
-  -> acc:felem s
-  -> pre:precomp s
-  -> len:size_t{0 < v len /\ v len % 64 = 0}
-  -> text:lbuffer uint8 len ->
-  Stack unit
-  (requires fun h ->
-    live h acc /\ live h pre /\ live h text /\
-    disjoint acc pre /\ disjoint acc text /\
-    precomp_inv_t h pre)
-  (ensures  fun h0 _ h1 ->
-    modifies1 acc h0 h1 /\ precomp_inv_t h1 pre /\
-    feval h1 acc == Vec.gf128_update_multi_mul_add (as_seq h0 text) (feval h0 acc) (get_r1 h0 pre))
-
-let gf128_update_multi_mul_add #s acc pre len text =
-  push_frame ();
-  let b4 = create_felem4 s in
-  let acc4 = create_felem4 s in
-  let tb = sub text 0ul 64ul in
-  load_acc acc tb acc4 b4;
-
-  let len1 = len -! 64ul in
-  let text1 = sub text 64ul len1 in
-  gf128_update_multi_mul_add_loop #s pre len1 text1 acc4 b4;
-
-  normalize4 acc acc4 pre;
-  pop_frame ()
-
-
-inline_for_extraction noextract
 val gf128_update_multi:
     #s:field_spec
   -> acc:felem s
@@ -459,12 +320,10 @@ val gf128_update_multi:
     precomp_inv_t h pre)
   (ensures  fun h0 _ h1 ->
     modifies1 acc h0 h1 /\ precomp_inv_t h1 pre /\
-    feval h1 acc == Vec.gf128_update_multi s (as_seq h0 text) (feval h0 acc) (get_r1 h0 pre))
+    feval h1 acc == Vec.gf128_update_multi (as_seq h0 text) (feval h0 acc) (get_r1 h0 pre))
 
 let gf128_update_multi #s acc pre len text =
-  match s with
-  | Vec.NI -> gf128_update_multi_add_mul acc pre len text
-  | Vec.PreComp -> gf128_update_multi_mul_add acc pre len text
+  gf128_update_multi_add_mul acc pre len text
 
 
 inline_for_extraction noextract
@@ -481,7 +340,7 @@ val gf128_update_vec:
     precomp_inv_t h pre)
   (ensures  fun h0 _ h1 ->
     modifies1 acc h0 h1 /\ precomp_inv_t h1 pre /\
-    feval h1 acc == Vec.gf128_update_vec s (as_seq h0 text) (feval h0 acc) (get_r1 h0 pre))
+    feval h1 acc == Vec.gf128_update_vec (as_seq h0 text) (feval h0 acc) (get_r1 h0 pre))
 
 let gf128_update_vec #s acc pre len text =
   let len0 = len /. 64ul *! 64ul in
@@ -508,7 +367,7 @@ let gf128_update #s ctx len text =
   let h0 = ST.get () in
   gf128_update_vec #s acc pre len text;
   let h1 = ST.get () in
-  Hacl.Spec.GF128.Equiv.gf128_update_vec_eq_lemma s (as_seq h0 text) (as_get_acc h0 ctx) (as_get_r h0 ctx);
+  Hacl.Spec.GF128.Equiv.gf128_update_vec_eq_lemma (as_seq h0 text) (as_get_acc h0 ctx) (as_get_r h0 ctx);
   assert (as_get_acc h1 ctx == S.gf128_update (as_seq h0 text) (as_get_acc h0 ctx) (as_get_r h0 ctx))
 
 
