code/gf128/Hacl.Spec.GF128.Vec.fst
@@ -11,8 +11,8 @@ open Spec.GaloisField
 module Scalar = Spec.GF128
 
 type gf128_spec =
+  | CT64
   | NI
-  | PreComp
 
 #reset-options "--z3rlimit 50 --max_fuel 0 --max_ifuel 0"
 
@@ -20,6 +20,8 @@ let _: squash (inversion gf128_spec) = allow_inversion gf128_spec
 
 let elem = Scalar.elem
 let gf128 = Scalar.gf128
+
+let elem2 = lseq elem 2
 
 let elem4 = lseq elem 4
 let fadd4 (a:elem4) (b:elem4) : elem4 = map2 fadd a b
@@ -47,8 +49,6 @@ let load_precompute_r (r:elem) : elem4 =
   let r4 = r `fmul_be` r3 in
   create4 r4 r3 r2 r
 
-
-//NI
 let gf128_update4_add_mul (pre:elem4) (b:lbytes 64) (acc:elem) : Tot elem =
   let acc = load_acc b acc in
   normalize4 pre acc
@@ -57,31 +57,14 @@ let gf128_update_multi_add_mul (text:bytes{0 < length text /\ length text % 64 =
   let pre = load_precompute_r r in
   repeat_blocks_multi #uint8 #elem 64 text (gf128_update4_add_mul pre) acc
 
+let gf128_update_multi (text:bytes{0 < length text /\ length text % 64 = 0}) (acc:elem) (r:elem) : elem =
+  gf128_update_multi_add_mul text acc r
 
-//Precomp
-let gf128_update4_mul_add (pre:elem4) (b:lbytes 64) (acc4:elem4) : Tot elem4 =
-  let r4 = create 4 pre.[0] in
-  fadd4 (fmul4 acc4 r4) (encode4 b)
-
-let gf128_update_multi_mul_add (text:bytes{0 < length text /\ length text % 64 = 0}) (acc:elem) (r:elem) : elem =
-  let pre = load_precompute_r r in
-  let acc = load_acc (Seq.slice text 0 64) acc in
-  let text = Seq.slice text 64 (length text) in
-  let acc = repeat_blocks_multi #uint8 #elem4 64 text (gf128_update4_mul_add pre) acc in
-  normalize4 pre acc
-
-
-
-let gf128_update_multi (alg:gf128_spec) (text:bytes{0 < length text /\ length text % 64 = 0}) (acc:elem) (r:elem) : elem =
-  match alg with
-  | NI -> gf128_update_multi_add_mul text acc r
-  | PreComp -> gf128_update_multi_mul_add text acc r
-
-let gf128_update_vec (alg:gf128_spec) (text:bytes) (acc:elem) (r:elem) : Tot elem =
+let gf128_update_vec (text:bytes) (acc:elem) (r:elem) : Tot elem =
   let len = length text in
   let len0 = len / 64 * 64 in
   let t0 = Seq.slice text 0 len0 in
-  let acc = if len0 > 0 then gf128_update_multi alg t0 acc r else acc in
+  let acc = if len0 > 0 then gf128_update_multi t0 acc r else acc in
 
   let t1 = Seq.slice text len0 len in
   Scalar.gf128_update t1 acc r
