Makefile
@@ -673,8 +673,8 @@ INTRINSIC_FLAGS = \
   -add-include 'Hacl_Hash_Blake2b_256:"libintvector.h"' \
   -add-include 'Hacl_Poly1305_256:"libintvector.h"' \
   \
-  -add-include 'Hacl_AES_128_NI:"libintvector.h"' \
-  -add-include 'Hacl_AES_256_NI:"libintvector.h"' \
+  -add-include 'Hacl_AES_128_CTR32_NI:"libintvector.h"' \
+  -add-include 'Hacl_AES_256_CTR32_NI:"libintvector.h"' \
   -add-include 'Hacl_AES_128_GCM_NI:"libintvector.h"' \
   -add-include 'Hacl_AES_256_GCM_NI:"libintvector.h"' \
   -add-include 'Hacl_Gf128_NI:"libintvector.h"'
